methods_same_signature withouth references to hyps

src/FJ/Semantics.v
@@ -212,12 +212,15 @@ Definition normal_form {X:Type} (R: relation X) (t: X) :=
   ~exists t', R t t'.
 
 
+Definition override (m: id) (D: ClassName) (Cs: [ClassName]) (C0: ClassName) :=
+    (forall Ds D0, mtype(m, D) = Ds ~> D0 -> (Ds = Cs /\ C0 = D0)).
+
 Inductive MType_OK : ClassName -> MethodDecl -> Prop :=
   | T_Method : forall C D C0 E0 xs Cs e0 Fs noDupfs K Ms noDupMds fargs m noDupFargs,
             nil extds (this :: xs) : (C :: Cs) |-- e0 : E0 ->
             E0 <: C0 ->
             find C CT = Some (CDecl C D Fs noDupfs K Ms noDupMds) ->
-            (forall Ds D0, mtype(m, D) = Ds ~> D0 -> Cs = Ds /\ C0 = D0) ->
+            override m D Cs C0 ->
             map fargType fargs = Cs ->
             refs fargs = xs ->
             MType_OK C (MDecl C0 m fargs noDupFargs e0).
